uf per
git-svn-id: svn://scm.gforge.inria.fr/svn/cfml@302 ba02c806-7d2b-4818-9a48-35b22e6bdc79

vacid/union_find.ml
@@ -11,7 +11,7 @@ let rec repr x =
 let create () = 
    ref Root
 
-let equiv x y =
+let same x y =
   repr x == repr y
 
 let union x y =
