vacid/union_find_proof.v
@@ -1,22 +1,97 @@
 Set Implicit Arguments.
-Require Import CFLib LibSet LibMap union_find_ml.
+Require Import CFLib LibSet LibMap LibRelation union_find_ml.
+
+
+(** LibRelation *)
+
+Module Import Rel := LibRelation.
+
+Definition single a b : binary A :=
+  fun x y => x = a /\ y = b.
+
+Record per A (R:binary A) :=
+ { per_sym : sym R;
+   per_trans : trans R }. 
+
+Definition per_dom A (R:binary A) :=
+  '{ x | R x x}.
+
+Lemma rel_eq_elim : forall A (R1 R2 : binary A), 
+  R1 = R2 -> (forall x y, R1 x y <-> R2 x y).
+Proof. intros. subst*. Qed.
+
+
+(*Lemma in_set : forall A (P:A->Prop) x,
+  x \in set_st P = P x.*)
+
+(** LibTactics *)
+
+Tactic Notation "applys_to" hyp(H1) "," hyp(H2) constr(E) :=
+  applys_to H1 E; applys_to H2 E.  
+
+(** CFTactics *)
+
+Ltac xapp_as_base spec args solver x :=
+  let cont tt := xapp_inst args solver in
+  xlet as x; 
+  [ xuntag tag_apply; xapp_core spec cont
+  | instantiate; xextract ].
+
+Tactic Notation "xapp" "as" ident(x) :=
+  xapp_as_base ___ (>>) ltac:(fun _ => idtac) x.
+Tactic Notation "xapp" "~" "as" ident(x) :=
+  xapp_as_base ___ (>>) ltac:(fun _ => xauto~) x.
+Tactic Notation "xapp" "*" "as" ident(x) :=
+  xapp_as_base ___ (>>) ltac:(fun _ => xauto*) x.
+nouveau dossier
+Tactic Notation "hextracts" :=
+  let E := fresh "TEMP" in hextract as E; subst_hyp E.
+
+Tactic Notation "xgos" :=
+  xgo; hsimpl.
+Tactic Notation "xgos" "~" :=
+  xgos; auto_tilde.
+Tactic Notation "xgos" "*" :=
+  xgos; auto_star.
+
+Tactic Notation "xapply" constr(H) :=
+  xapply_local H. 
+Tactic Notation "xapplys" constr(H) :=
+  xapply_local H; [ hcancel | hsimpl ].
+
+Tactic Notation "xapplys" "~" constr(H) :=
+  xapplys H; auto_tilde.
+Tactic Notation "xapplys" "*" constr(H) :=
+  xapplys H; auto_star.
 
 
 Instance content_inhab : Inhab content.
 Proof. typeclass. Qed.
 Hint Resolve content_inhab.
 
-Notation "x \indom' E" := (@is_in _ (set _) _ x (@dom _ (set loc) _ E)) 
-  (at level 39) : container_scope.
-Notation "x \notindom' E" := (x \notin ((dom E) : set _)) 
-  (at level 39) : container_scope.
 
+(** CFPrim *)
 
-(****************************************************)
-(** Reflexive-symmetric-transitive closure *) 
+Axiom ml_ref_spec_group : forall a,
+  Spec ml_ref (v:a) |R>> forall (M:map loc a),
+    R (Group (Ref Id) M) (fun l => Group (Ref Id) (M\(l:=v)) \* [l\notindom' M]).
 
-(** Recall that [binary A] is the type of binary 
-    relations over A, defined as [A->A->Prop]. *)
+Axiom ml_get_spec_group : forall a,
+  Spec ml_get (l:loc) |R>> forall (M:map loc a),   
+    Inhab a -> l \indom M ->
+    keep R (Group (Ref Id) M) (\= M\(l)).
+
+Axiom ml_set_spec_group : forall a, 
+  Spec ml_set (l:loc) (v:a) |R>> forall (M:map loc a), 
+    Inhab a -> l \indom M ->
+    R (Group (Ref Id) M) (# Group (Ref Id) (M\(l:=v))).
+
+(** Other *)
+
+Lemma case_classic_l : forall P Q, P \/ Q -> (P \/ (~ P /\ Q)).
+Proof. intros. tautoB P Q. Qed.
+
+(*
 
 Inductive closure (A:Type) (R:binary A) : binary A :=
   | closure_step : forall x y,
@@ -29,32 +104,117 @@ Inductive closure (A:Type) (R:binary A) : binary A :=
       closure R x y -> closure R y z -> closure R x z.
 
 
+Hint Constructors closure.
+Lemma closure_le : forall A (R1 R2 : binary A),
+  rel_le R1 R2 -> rel_le (closure R1) (closure R2).
+Proof. unfolds rel_le, pred_le. introv Le H. induction* H. Qed.
+*)
+
+(** Maps *)
+
+Notation "x \indom' E" := (@is_in _ (set _) _ x (@dom _ (set loc) _ E)) 
+  (at level 39) : container_scope.
+Notation "x \notindom' E" := (x \notin ((dom E) : set _)) 
+  (at level 39) : container_scope.
+
+Axiom map_indom_update_inv : forall A `{Inhab B} (m:map A B) (i j:A) (v:B),
+  j \indom (m\(i:=v)) -> (j = i \/ j \indom m).
+Axiom map_indom_update_already : forall A `{Inhab B} (m:map A B) (i j:A) (v:B),
+  j \indom m -> j \indom (m\(i:=v))
+
+Axiom binds_def : forall A `{Inhab B} (M:map A B) x v,
+  binds M x v = (x \indom M /\ M\(x) = v).
+Axiom binds_inv : forall A `{Inhab B} (M:map A B) x v,
+  binds M x v -> (x \indom M /\ M\(x) = v).
+Axiom binds_prove : forall A `{Inhab B} (M:map A B) x v,
+  x \indom M -> M\(x) = v -> binds M x v.
+
+Axiom binds_update_neq : forall A i j `{Inhab B} v w (M:map A B),
+  j \notindom' M -> binds M i v -> binds (M\(j:=w)) i v.
+Axiom binds_update_eq : forall A i `{Inhab B} v (M:map A B),
+  binds (M\(i:=v)) i v.
+
+Axiom binds_inj : forall A i `{Inhab B} v1 v2 (M:map A B),
+  binds M i v1 -> binds M i v2 -> v1 = v2.
+
+(*
+Axiom binds_update_rem : forall A i j `{Inhab B} v w (M:map A B),
+  j \notindom' M -> binds (M\(j:=w)) i v -> binds M i v.
+Hint Resolve binds_update_rem.
+
+Lemma is_repr_rem_node : forall M r c x y,
+  r \notin (dom M:set _) -> is_repr (M\(r:=c)) x y -> is_repr M x y.
+Proof. introv N H. induction H; constructors*. Qed. 
+*)
+
+Axiom binds_get : forall A `{Inhab B} (M:map A B) x v,
+  binds M x v -> M\(x) = v.
+Axiom binds_dom : forall A `{Inhab B} (M:map A B) x v,
+  binds M x v -> x \indom M.
+
+Axiom dom_update_notin : forall A i `{Inhab B} v (M:map A B),
+  i \notindom' M -> dom (M\(i:=v)) = dom M \u \{i}.
+
+Axiom binds_index : forall A i `{Inhab B} v (M:map A B),
+  binds M i v -> index M i.
+
+Axiom binds_update_neq' : forall A i j `{Inhab B} v w (M:map A B),
+  i <> j -> binds M i v -> binds (M\(j:=w)) i v.
+
+
+Global Opaque binds_inst. 
+
+(* todo: bug de congruence *)
+
+
 (****************************************************)
-(** Graph structure *)
+(** Reflexive-symmetric-transitive closure *) 
 
-(** A graph has nodes and edges, which are pairs of nodes. *)
+(** Recall that [binary A] is the type of binary 
+    relations over A, defined as [A->A->Prop]. *)
 
-Record graph A := graph_of { 
-  nodes : set A;
-  edges : set (A*A) }.
+Inductive stclosure (A:Type) (R:binary A) : binary A :=
+  | stclosure_step : forall x y,
+      R x y -> stclosure R x y
+  | stclosure_sym : forall x y, 
+      stclosure R x y -> stclosure R y x
+  | stclosure_trans : forall y x z,
+      stclosure R x y -> stclosure R y z -> stclosure R x z.
 
-(** The functions [add_node] and [add_edge] can be used to
-    augment a given graph. *)
+Hint Resolve stclosure_step stclosure_sym stclosure_trans.
 
-Definition add_node A (G:graph A) x :=
-  graph_of (nodes G \u \{x}) (edges G).
+Lemma stclosure_le : forall A (R1 R2 : binary A),
+  rel_le R1 R2 -> rel_le (stclosure R1) (stclosure R2).
+Proof. unfolds rel_le, pred_le. introv Le H. induction* H. Qed.
 
-Definition add_edge A (G:graph A) x y :=
-  graph_of (nodes G) (edges G \u \{(x,y)}).
 
-(** [connected G x y] indicates that the nodes [x] and [y]
-    belong to the same connected component in [G]. 
-    A connected component is defined as the reflexive-
-    symmetric-transitive closure of the edges. *)
 
-Definition connected A (G:graph A) x y :=
+(** Extension of an per [B] with a node [z] *)
 
-  closure (fun x y => (x,y) \in edges G) x y.
+Definition add_node A (B:binary A) (z:A) :=
+  Rel.union B (single z z).
+
+(** Extension of an per [B] with an edge between [x] and [y] *)
+
+Definition add_edge A (B:binary A) (x y:A) :=
+  stclosure (Rel.union B (single x y)).
+
+Lemma add_edge_already : forall A (B:binary A) x y,
+  per B -> B x y -> add_edge B x y = B.
+Proof.
+  introv (_&_&E). extens. intros a b. unfold connected. simpls.
+  iff (Ia&Ib&R); splits~.
+  clear Ia Ib. induction R; intros.
+    destruct (in_union_inv H) as [|M].
+      eauto.
+      rewrite (in_single_eq) in M. inverts~ M.  
+    eauto.
+    eauto.
+    eauto.
+  applys closure_le R. intros u v M. apply in_union_l. eauto.
+Qed.
+
+
 
 
 (****************************************************)
@@ -83,13 +243,16 @@ Definition is_forest M :=
 Definition is_equiv M x y :=
   exists r, is_repr M x r /\ is_repr M y r. 
 
-(** [UF G] is a heap predicate that corresponds to a set of 
+(** [UF B] is a heap predicate that corresponds to a set of 
     cells describing the union-find structure associated with
-    the graph [G], where the nodes of [G] are of type [loc] *)
-    
-Definition UF (G:graph loc) : hprop :=
+    the PER [R], which is a binary relation over locations. *)
+
+Definition UF (B:binary loc) : hprop :=
   Hexists (M:map loc content), Group (Ref Id) M \*
-    [ is_forest M /\ dom M = nodes G /\ is_equiv M = connected G ].
+    [ per B /\
+      is_forest M /\
+      dom M = per_dom B /\
+      is_equiv M = B ].
 
 
 (****************************************************)
@@ -98,46 +261,28 @@ Definition UF (G:graph loc) : hprop :=
 Hint Constructors is_repr.
 Hint Unfold is_equiv.
 
-
-
 Tactic Notation "rew_map" "~" := 
   rew_map; auto_tilde.
 
-
-Axiom map_indom_inv : forall A `{Inhab B} (m:map A B) (i j:A) (v:B),
-  j \indom (m\(i:=v)) -> (j = i \/ j \indom m).
-
-Lemma case_classic_l : forall P Q, P \/ Q -> (P \/ (~ P /\ Q)).
-Proof. intros. tautoB P Q. Qed.
-
-
-Axiom binds_def : forall A `{Inhab B} (M:map A B) x v,
-  binds M x v = (x \indom M /\ M\(x) = v).
-Axiom binds_inv : forall A `{Inhab B} (M:map A B) x v,
-  binds M x v -> (x \indom M /\ M\(x) = v).
-Axiom binds_prove : forall A `{Inhab B} (M:map A B) x v,
-  x \indom M -> M\(x) = v -> binds M x v.
-
-Axiom binds_update_neq : forall A i j `{Inhab B} v w (M:map A B),
-  j \notindom' M -> binds M i v -> binds (M\(j:=w)) i v.
-Axiom binds_update_eq : forall A i `{Inhab B} v (M:map A B),
-  binds (M\(i:=v)) i v.
-
-Axiom binds_inj : forall A i `{Inhab B} v1 v2 (M:map A B),
-  binds M i v1 -> binds M i v2 -> v1 = v2.
-
+Hint Resolve binds_index.
+Hint Resolve binds_update_neq'.
 
 Hint Resolve binds_update_neq binds_update_eq.
 
-Axiom ml_ref_spec_group : forall a,
-  Spec ml_ref (v:a) |R>> forall (M:map loc a),
-    R (Group (Ref Id) M) (fun l => Group (Ref Id) (M\(l:=v)) \* [l\notindom' M]).
+
+Lemma is_equiv_iff_same_repr : forall M x y rx ry,
+  is_repr M x rx -> is_repr M y ry ->
+  ((rx = ry) <-> is_equiv M x y).
+Proof. 
+  introv Rx Ry. iff H (r&Rx'&Ry'). subst*.
+  applys (eq_trans r); applys is_repr_inj; eauto.
+Qed.
 
 
 (****************************************************)
 (** Lemmas *)
 
-Global Opaque binds_inst. (* todo: bug de congruence *)
+(** Properties of [is_repr] *)
 
 Lemma is_repr_inj : forall r1 r2 M x,
   is_repr M x r1 -> is_repr M x r2 -> r1 = r2.
@@ -145,13 +290,8 @@ Proof.
   introv H. gen r2. induction H; introv H'; inverts H'; auto_false.
   forwards~ E: binds_inj H1 H. inverts~ E.
 Qed.
-(*
- inverts H'.
-    auto. 
-    forwards~: binds_inj H H0. false.
-  inverts H'. 
-    forwards~: binds_inj H1 H. false.  
-    forwards~ E: binds_inj H1 H. inverts E. apply~ IHis_repr.*)
+
+Implicit Arguments is_repr_inj [ ].
 
 Lemma is_equiv_refl : forall M x, 
   x \indom M -> is_forest M -> is_equiv M x x.
@@ -161,8 +301,6 @@ Lemma is_equiv_sym : forall M,
   sym (is_equiv M).
 Proof. intros M x y (r&Hx&Hy). eauto. Qed.
 
-Implicit Arguments is_repr_inj [ ].
-
 Lemma is_equiv_trans : forall M,
   trans (is_equiv M).
 Proof.
@@ -170,73 +308,80 @@ Proof.
   forwards: is_repr_inj r1 r2; eauto. subst*.
 Qed.
 
+Lemma is_repr_in_dom_l : forall M x r, 
+  is_repr M x r -> x \indom M.
+Proof. introv H. inverts H; apply* binds_dom. Qed. 
+
+Lemma is_repr_in_dom_r : forall M x r, 
+  is_repr M x r -> r \indom M.
+Proof. introv H. induction H. apply* binds_dom. auto. Qed. 
+
+Lemma is_repr_binds_root : forall M x r, 
+  is_repr M x r -> binds M r Root.
+Proof. introv H. induction~ H. Qed.
+
+Hint Resolve is_repr_in_dom_l is_repr_in_dom_r is_repr_binds_root.
+
+(** General lemmas *)
+
 Lemma is_repr_add_node : forall M r c x y,
   r \notin (dom M:set _) -> is_repr M x y -> is_repr (M\(r:=c)) x y.
 Proof. introv N H. induction H; constructors*. Qed. 
 
-(*
-Axiom binds_update_rem : forall A i j `{Inhab B} v w (M:map A B),
-  j \notindom' M -> binds (M\(j:=w)) i v -> binds M i v.
-Hint Resolve binds_update_rem.
-
-Lemma is_repr_rem_node : forall M r c x y,
-  r \notin (dom M:set _) -> is_repr (M\(r:=c)) x y -> is_repr M x y.
-Proof. introv N H. induction H; constructors*. Qed. 
-*)
-
-Axiom binds_get : forall A `{Inhab B} (M:map A B) x v,
-  binds M x v -> M\(x) = v.
-Axiom binds_dom : forall A `{Inhab B} (M:map A B) x v,
-  binds M x v -> x \indom M.
-
-Lemma is_repr_in_dom : forall M x r, 
-  is_repr M x r -> x \indom M.
-Proof. introv H. inverts H; apply* binds_dom. Qed. 
-
-Lemma rel_eq_elim : forall A (R1 R2 : binary A), 
-  R1 = R2 -> (forall x y, R1 x y <-> R2 x y).
-Proof. intros. subst*. Qed.
-
-
-Axiom dom_update_notin : forall A i `{Inhab B} v (M:map A B),
-  i \notindom' M -> dom (M\(i:=v)) = dom M \u \{i}.
-
-Tactic Notation "applys_to" hyp(H1) "," hyp(H2) constr(E) :=
-  applys_to H1 E; applys_to H2 E.  
-(*
-Lemma is_repr_added_node : forall M x z,
-  z \notindom' M -> is_repr (M\(z:=Root)) x z -> x = z.
+Lemma node_not_root : forall r x M y,
+  binds M r Root -> is_repr M x (Node y) -> x <> r.
 Proof.
-  introv D Rx. inverts~ Rx.
 Qed.
 
-*)
-Lemma inv_add_node : forall M G z,
-  is_forest M ->
-  dom M = nodes G ->
-  is_equiv M = connected G ->
-  z \notindom' M -> 
-  is_equiv (M\(z:=Root)) = connected (add_node G z).
+Lemma points_indom : forall x M y,
+  binds M x (Node y) -> is_forest M -> y \indom M.
 Proof.
-  introv FM DM EM D. extens. intros x y.
-  lets EQ: (rel_eq_elim (rm EM) x y). iff (r&Rx&Ry) H.
-  (* -> *)
-  unfolds. simpl. rewrite <- DM. 
-  lets Mx: is_repr_in_dom Rx. lets My: is_repr_in_dom Ry.
-  rewrite dom_update_notin in Mx,My; auto. splits~.
-  apply EQ. tests (r = z).
-    exists z. skip.
-    skip.  (* todo! *)
-  (* <- *)
-  lets H': H. unfolds in H'. simpl in H'. skip.
 Qed.
+
+Hint Resolve node_not_root points_indom.
+ 
+(** Lemmas for 'create' function *)
 
 Lemma is_forest_add_node : forall M r,
   is_forest M -> r \notindom' M -> is_forest (M\(r:=Root)).
 Proof.
-  introv FM Dr. intros x Dx. destruct (map_indom_inv Dx).
+  introv FM Dr. intros x Dx. destruct (map_indom_update_inv Dx).
     subst*.
     forwards* [y Ry]: FM x. exists y. apply* is_repr_add_node.
+Qed.
+
+Lemma inv_add_node : forall M B z,
+  is_forest M ->
+  dom M = rel_dom B ->
+  is_equiv M = B ->
+  z \notindom' M -> 
+  is_equiv (M\(z:=Root)) = add_node B z.
+Proof.
+Qed.
+
+(** Lemmas for 'union' function *)
+
+Lemma is_forest_add_edge : forall M rx ry,
+  is_forest M -> binds M rx Root -> binds M ry Root -> rx <> ry ->
+  is_forest (M\(rx:=Node ry)).
+Proof.
+  introv FM Bx By Neq. intros x D. rewrite* dom_update_in in D.
+  forwards~ [r R]: FM x. tests (r = rx) as C.
+  exists ry. induction R.
+    eauto.
+    cuts*: (x <> r). intro_subst. congruence.
+  exists r. gen C. induction R; intros.
+    eauto.
+    cuts*: (x<>rx). congruence.
+Qed.
+
+Lemma inv_add_edge : forall M G a ra b rb,
+  per B ->
+  is_equiv M = B ->
+  is_repr M a ra ->
+  is_repr M b rb ->
+  is_equiv (M\(rx:=Node ry)) = add_edge B a b.
+Proof.
 Qed.
 
 
@@ -245,29 +390,6 @@ Qed.
 
 (*--------------------------------------------------*)
 (** Function [repr] *)
-
-Axiom ml_get_spec_group : forall a,
-  Spec ml_get (l:loc) |R>> forall (M:map loc a),   
-    Inhab a -> l \indom M ->
-    keep R (Group (Ref Id) M) (\= M\(l)).
-
-
-Tactic Notation "xgos" :=
-  xgo; hsimpl.
-Tactic Notation "xgos" "~" :=
-  xgos; auto_tilde.
-Tactic Notation "xgos" "*" :=
-  xgos; auto_star.
-
-Tactic Notation "xapply" constr(H) :=
-  xapply_local H. 
-Tactic Notation "xapplys" constr(H) :=
-  xapply_local H; [ hcancel | hsimpl ].
-
-Tactic Notation "xapplys" "~" constr(H) :=
-  xapplys H; auto_tilde.
-Tactic Notation "xapplys" "*" constr(H) :=
-  xapplys H; auto_star.
 
 Lemma repr_spec :
   Spec repr x |R>> forall M,
@@ -290,10 +412,9 @@ Hint Extern 1 (RegisterSpec repr) => Provide repr_spec.
 (*--------------------------------------------------*)
 (** Function [create] *)
 
-
 Lemma create_spec :
-  Spec create () |R>> forall G,
-    R (UF G) (fun r => UF (add_node G r)).
+  Spec create () |R>> forall B,
+    S (UF B) (fun r => [r \notin (rel_dom B)] \* UF (Rel.union B (single r r))).
 Proof.
   xcf. intros. unfold UF. xextract as M (FM&DM&EM).
   xapp_spec ml_ref_spec_group.
@@ -307,43 +428,12 @@ Hint Extern 1 (RegisterSpec create) => Provide create_spec.
 
 
 (*--------------------------------------------------*)
-(** Function [equiv] *)
+(** Function [same] *)
 
-(*
-Lemma indom_from_innodes : forall x G M,
-  dom M = nodes G -> x \in nodes G -> x \indom' M.
-Proof. introv H D. rewrite H. auto. Qed.
-Hint Resolve indom_from_innodes.
-*)
-
-Ltac xapp_as_base spec args solver x :=
-  let cont tt := xapp_inst args solver in
-  xlet as x; 
-  [ xuntag tag_apply; xapp_core spec cont
-  | instantiate; xextract ].
-
-Tactic Notation "xapp" "as" ident(x) :=
-  xapp_as_base ___ (>>) ltac:(fun _ => idtac) x.
-Tactic Notation "xapp" "~" "as" ident(x) :=
-  xapp_as_base ___ (>>) ltac:(fun _ => xauto~) x.
-Tactic Notation "xapp" "*" "as" ident(x) :=
-  xapp_as_base ___ (>>) ltac:(fun _ => xauto*) x.
-nouveau dossier
-Tactic Notation "hextracts" :=
-  let E := fresh "TEMP" in hextract as E; subst_hyp E.
-
-Lemma is_equiv_iff_same_repr : forall M x y rx ry,
-  is_repr M x rx -> is_repr M y ry ->
-  ((rx = ry) <-> is_equiv M x y).
-Proof. 
-  introv Rx Ry. iff H (r&Rx'&Ry'). subst*.
-  applys (eq_trans r); applys is_repr_inj; eauto.
-Qed.
-
-Lemma equiv_spec :
-  Spec equiv x y |R>> forall G, 
-    x \in (nodes G) -> y \in (nodes G) ->
-    keep R (UF G) (\= istrue(connected G x y)).
+Lemma same_spec :
+  Spec same x y |R>> forall B, 
+    x \in (rel_dom B) -> y \in (rel_dom B) ->
+    keep R (UF B) (\= istrue (B x y)).
 Proof.
   xcf. introv Dx Dy. unfold UF. xextract as M (FM&DM&EM).
   rewrite <- DM in *. clear DM.
@@ -358,93 +448,23 @@ Hint Extern 1 (RegisterSpec equiv) => Provide equiv_spec.
 (*--------------------------------------------------*)
 (** Function [union] *)
 
-Axiom ml_set_spec_group : forall a, 
-  Spec ml_set (l:loc) (v:a) |R>> forall (M:map loc a), 
-    Inhab a -> l \indom M ->
-    R (Group (Ref Id) M) (# Group (Ref Id) (M\(l:=v))).
-
-Lemma is_repr_in_dom' : forall M x r, 
-  is_repr M x r -> r \indom M.
-Proof. introv H. induction H. apply* binds_dom. auto. Qed. 
-
-Lemma is_repr_binds_root : forall M x r, 
-  is_repr M x r -> binds M r Root.
-Proof. introv H. induction~ H. Qed.
-
-Axiom binds_index : forall A i `{Inhab B} v (M:map A B),
-  binds M i v -> index M i.
-Hint Resolve binds_index.
-
-Axiom binds_update_neq' : forall A i j `{Inhab B} v w (M:map A B),
-  i <> j -> binds M i v -> binds (M\(j:=w)) i v.
-Hint Resolve binds_update_neq'.
-
-
-Hint Resolve is_repr_in_dom.
-Lemma is_forest_update : forall M rx ry,
-  is_forest M -> binds M rx Root -> binds M ry Root -> rx <> ry ->
-  is_forest (M\(rx:=Node ry)).
-Proof.
-  introv FM Bx By Neq. intros x D. rewrite* dom_update_in in D.
-  forwards~ [r R]: FM x. tests (r = rx) as C.
-  exists ry. induction R.
-    eauto.
-    cuts*: (x <> r). intro_subst. congruence.
-  exists r. gen C. induction R; intros.
-    eauto.
-    cuts*: (x<>rx). congruence.
-Qed.
-
-
-  
-
-Lemma inv_add_edge : forall M G x rx y ry,
-  is_equiv M = connected G ->
-  is_repr M x rx ->
-  is_repr M y ry ->
-  is_equiv (M\(rx:=Node ry)) = connected (add_edge G x y).
-Admitted.
-
-
-Hint Constructors closure.
-Lemma closure_le : forall A (R1 R2 : binary A),
-  rel_le R1 R2 -> rel_le (closure R1) (closure R2).
-Proof. unfolds rel_le, pred_le. introv Le H. induction* H. Qed.
-
-
-Lemma connected_already : forall A (G:graph A) x y,
-  connected G x y ->
-  connected (add_edge G x y) = connected G.
-Proof.
-  introv (_&_&E). extens. intros a b. unfold connected. simpls.
-  iff (Ia&Ib&R); splits~.
-  clear Ia Ib. induction R; intros.
-    destruct (in_union_inv H) as [|M].
-      eauto.
-      rewrite (in_single_eq) in M. inverts~ M.  
-    eauto.
-    eauto.
-    eauto.
-  applys closure_le R. intros u v M. apply in_union_l. eauto.
-Qed.
-
 Lemma union_spec :
-  Spec union x y |R>> forall G,
-    x \in (nodes G) -> y \in (nodes G) ->
-    R (UF G) (# UF (add_edge G x y)).
+  Spec union x y |R>> forall B,
+    x \in (rel_dom B) -> y \in (rel_dom B) ->
+    R (UF B) (# UF (stclosure (Rel.union B (single x y)))).
 Proof.
   xcf. introv Dx Dy. unfold UF. xextract as M (FM&DM&EM).
   rewrite <- DM in *. clear DM.
   xapp~ as rx. intros Rx. xapp~ as ry. intros Ry.
   xapps. xif.
   (* case [rx <> ry] *)
-  xapp_spec~ ml_set_spec_group. apply* is_repr_in_dom'.
+  xapp_spec~ ml_set_spec_group. apply* is_repr_in_dom_r.
   hsimpl. splits.
-    apply* is_forest_update; apply* is_repr_binds_root.  
+    apply* is_forest_add_edge; apply* is_repr_binds_root.  
     rewrite~ dom_update_in. forwards*: is_repr_binds_root Rx.
     apply* inv_add_edge.
   (* case [rx = ry] *)
-  xrets. splits~. rewrite~ connected_already. rewrite* <- EM. 
+  xrets. splits~. rewrite~ inv_add_no_edge. rewrite* <- EM. 
 Admitted.
 
 Hint Extern 1 (RegisterSpec union) => Provide union_spec.
@@ -452,6 +472,8 @@ Hint Extern 1 (RegisterSpec union) => Provide union_spec.
 
 
 
+---------------
+---------------
 ---------------
 
 (*
@@ -480,3 +502,46 @@ Lemma is_equiv_add_node : forall M r x y,
   is_equiv (M\(r:=Root)) x y = (is_equiv M x y \/ (x = r /\ y = r)).
 Admitted.
 *)
+
+(****************************************************)
+(** Graph structure *)
+
+(** A graph has nodes and edges, which are pairs of nodes. *)
+
+Record graph A := graph_of { 
+  nodes : set A;
+  edges : set (A*A) }.
+
+(** The functions [add_node] and [add_edge] can be used to
+    augment a given graph. *)
+
+Definition add_node A (G:graph A) x :=
+  graph_of (nodes G \u \{x}) (edges G).
+
+Definition add_edge A (G:graph A) x y :=
+  graph_of (nodes G) (edges G \u \{(x,y)}).
+
+(** [connected G x y] indicates that the nodes [x] and [y]
+    belong to the same connected component in [G]. 
+    A connected component is defined as the reflexive-
+    symmetric-transitive closure of the edges. *)
+
+Definition connected A (G:graph A) x y :=
+  closure (fun x y => (x,y) \in edges G) x y.
+
+(*-----
+Lemma is_repr_added_node : forall M x z,
+  z \notindom' M -> is_repr (M\(z:=Root)) x z -> x = z.
+Proof.
+  introv D Rx. inverts~ Rx.
+Qed.
+
+
+
+(*
+Lemma indom_from_innodes : forall x G M,
+  dom M = nodes G -> x \in nodes G -> x \indom' M.
+Proof. introv H D. rewrite H. auto. Qed.
+Hint Resolve indom_from_innodes.
+*)
+
